Remove more about annotations

Hoare/Hoare.thy
@@ -460,10 +460,6 @@ definition magic_filter :: "8 word list \<Rightarrow> bool" where
    (lst = word_rsplit a @ word_rsplit b) \<longrightarrow>
    hash2 a b \<noteq> 0)"
 
-definition no_assertion :: "constant_ctx \<Rightarrow> bool"
-  where "no_assertion c == (\<forall> pos. program_annotation (cctx_program c) pos = [])
-    \<and> cctx_hash_filter c = magic_filter"
-
 definition failed_for_reasons :: "failure_reason set \<Rightarrow> instruction_result \<Rightarrow> bool"
 where
 "failed_for_reasons allowed r =
@@ -477,15 +473,11 @@ definition triple ::
  "network \<Rightarrow> failure_reason set \<Rightarrow> (state_element set \<Rightarrow> bool) \<Rightarrow> (int * inst) set \<Rightarrow> (state_element set \<Rightarrow> bool) \<Rightarrow> bool"
 where
   "triple net allowed_failures pre insts post ==
-    \<forall> co_ctx presult rest stopper. no_assertion co_ctx \<longrightarrow>
+    \<forall> co_ctx presult rest stopper.
        (pre ** code insts ** rest) (instruction_result_as_set co_ctx presult) \<longrightarrow>
        (\<exists> k.
          ((post ** code insts ** rest) (instruction_result_as_set co_ctx (program_sem stopper co_ctx k net presult)))
          \<or> failed_for_reasons allowed_failures (program_sem stopper co_ctx k net presult))"
-
-lemma no_assertion_pass [simp] : "no_assertion co_ctx \<Longrightarrow> check_annotations v co_ctx"
-apply(simp add: no_assertion_def check_annotations_def)
-done
 
 lemma pure_sep [simp] : "(((\<langle> b \<rangle>) ** rest) s) = (b \<and> rest s)"
   by ( simp add: sep_conj_def pure_def emp_def )
@@ -655,6 +647,16 @@ apply(auto simp add: contexts_as_set_def constant_ctx_as_set_def variable_ctx_as
       balance_as_set_def log_as_set_def data_sent_as_set_def ext_program_as_set_def)
 done
 
+lemma codeElmInInstructionResult [simp] :
+ "CodeElm (pos, i) \<in> instruction_result_as_set co_ctx presult =
+   ((program_content (cctx_program co_ctx) pos = Some i) \<or>
+   (program_content (cctx_program co_ctx) pos = None) \<and> i = Misc STOP)"
+by(case_tac presult; auto simp add: contexts_as_set_def constant_ctx_as_set_def variable_ctx_as_set_def
+   program_as_set_def stack_as_set_def memory_as_set_def storage_as_set_def
+   balance_as_set_def log_as_set_def data_sent_as_set_def ext_program_as_set_def
+   instruction_result_as_set_def)
+
+
 lemma codeElmEquiv [simp] :
   "CodeElm (pos, i) \<in> contexts_as_set va_ctx co_ctx =
    ((program_content (cctx_program co_ctx) pos = Some i) \<or>
@@ -733,7 +735,6 @@ lemma triple_continue:
       \<or> failed_for_reasons allowed (program_sem s co_ctx (k + l) net presult))"
 apply(simp add: triple_def)
 apply(drule_tac x = co_ctx in spec)
-apply(simp)
 apply(drule_tac x = "program_sem s co_ctx k net presult" in spec)
 apply(drule_tac x = rest in spec)
 apply(simp)
@@ -782,44 +783,84 @@ lemma composition:
   apply (subst (asm) triple_def[where pre=P])
   apply clarsimp
   apply (rename_tac co_ctx presult rest stopper)
-  apply(drule_tac x = "co_ctx" in spec, simp)
+  apply(drule_tac x = "co_ctx" in spec)
   apply(drule_tac x = "presult" in spec)
-  apply(drule_tac x = "code (cR - cL) ** rest" in spec; simp add: code_more)
+  apply(drule_tac x = "code (cR - cL) ** rest" in spec)
+  apply clarsimp
   apply (erule impE)
-   apply clarsimp
-   apply (rule conjI, blast)+
-   apply (erule_tac P="P \<and>* rest" in back_subst)
+   apply(rule conjI)
+    apply (thin_tac "(_ \<and>* _) _")+
+    apply clarsimp
+    apply(subgoal_tac "CodeElm (pos, i) \<in> instruction_result_as_set co_ctx presult")
+     apply clarsimp
+    apply(subgoal_tac "CodeElm (pos, i) \<in> {CodeElm (pos, i) |pos i. (pos, i) \<in> cL \<or> (pos, i) \<in> cR}")
+     apply blast
+    apply blast
+   apply(rule conjI)
+    apply clarsimp
+    apply(subgoal_tac "CodeElm (pos, i) \<in> {CodeElm (pos, i) |pos i. (pos, i) \<in> cL \<or> (pos, i) \<in> cR}")
+     apply(subgoal_tac "CodeElm (pos,i ) \<in> instruction_result_as_set co_ctx presult")
+      apply clarsimp
+     apply blast
+    apply blast
+   apply(subgoal_tac "(instruction_result_as_set co_ctx presult - {CodeElm (pos, i) |pos i. (pos, i) \<in> cL \<or> (pos, i) \<in> cR})
+    = (instruction_result_as_set co_ctx presult - {CodeElm (pos, i) |pos i. (pos, i) \<in> cL} -
+         {CodeElm (pos, i) |pos i. (pos, i) \<in> cR \<and> (pos, i) \<notin> cL})")
+    apply simp
    apply blast
   apply(drule_tac x = stopper in spec)
-  apply clarsimp
- apply (clarsimp simp add: triple_def)
-  apply(drule_tac x = "co_ctx" in spec, simp)
-  apply(drule_tac x = "program_sem stopper co_ctx k net presult" in spec)
+  apply(erule exE)
+  apply (subst (asm) triple_def[where pre=Q])
+  apply(drule_tac x = "co_ctx" in spec)
+  apply(drule_tac x = "(program_sem stopper co_ctx k net presult)" in spec)
   apply(drule_tac x = "code (cL - cR) ** rest" in spec)
-  apply (erule disjE)
-   prefer 2
-   apply auto[1]
-  apply clarsimp
-  apply (erule impE)
-    apply (rule conjI, blast)+
-    apply (erule_tac P="Q \<and>* rest" in back_subst)
-    apply blast
+  apply(erule disjE)
    apply(drule_tac x = stopper in spec)
+   apply (erule impE)
+    apply clarsimp
+    apply(rule conjI)
+     apply (thin_tac "c = _")
+     apply (thin_tac "_ \<subseteq> instruction_result_as_set co_ctx presult")
+     apply (thin_tac "(_ \<and>* _) _")
+     apply clarsimp
+     apply(subgoal_tac "CodeElm(pos,i) \<in> instruction_result_as_set co_ctx (program_sem stopper co_ctx k net presult)")
+      apply clarsimp
+     apply(case_tac "(pos, i) \<in> cL")
+      apply blast
+     apply blast
+    apply(rule conjI)
+     apply blast
+    apply(subgoal_tac "(instruction_result_as_set co_ctx (program_sem stopper co_ctx k net presult) -
+         {CodeElm (pos, i) |pos i. (pos, i) \<in> cL} -
+         {CodeElm (pos, i) |pos i. (pos, i) \<in> cR \<and> (pos, i) \<notin> cL}) =
+         (instruction_result_as_set co_ctx (program_sem stopper co_ctx k net presult) -
+         {CodeElm (pos, i) |pos i. (pos, i) \<in> cR} -
+         {CodeElm (pos, i) |pos i. (pos, i) \<in> cL \<and> (pos, i) \<notin> cR})")
+     apply simp
+    apply blast
+   apply(erule exE)
+   apply(rename_tac k l)
+   apply(rule_tac x = "k + l" in exI)
+   apply(erule disjE)
+   apply(rule disjI1)
+   apply (rule conjI)
+    apply (thin_tac "(_ \<and>* _) _")+
+    apply clarsimp
+    apply(subgoal_tac "CodeElm (pos,i) \<in> instruction_result_as_set co_ctx presult")
+     apply clarsimp
+    apply blast
    apply clarsimp
-  apply (erule disjE)
-   prefer 2
-   apply auto[1]
-  apply clarsimp
-  apply (rename_tac k m)
-  apply(rule_tac x = "k + m" in exI)
-  apply (rule disjI1)
-  apply (rule conjI)
-   apply (thin_tac "(_ \<and>* _) _")+
-   apply (thin_tac "_ \<subseteq> instruction_result_as_set co_ctx presult")
-   apply (erule (1) set_compr_double_neg_subseteq)
-  apply (erule back_subst[where P="R \<and>* _"])
-  apply blast
- done
+   apply(subgoal_tac "
+   (instruction_result_as_set co_ctx (program_sem stopper co_ctx (k + l) net presult) -
+         {CodeElm (pos, i) |pos i. (pos, i) \<in> cR} -
+         {CodeElm (pos, i) |pos i. (pos, i) \<in> cL \<and> (pos, i) \<notin> cR}) =
+   (instruction_result_as_set co_ctx (program_sem stopper co_ctx (k + l) net presult) -
+         {CodeElm (pos, i) |pos i. (pos, i) \<in> cL \<or> (pos, i) \<in> cR})")
+    apply simp
+   apply blast
+  by auto
+
+
 (** Frame **)
 
 lemma frame:
@@ -828,7 +869,6 @@ lemma frame:
   apply clarsimp
   subgoal for co_ctx presult rest stopper
   apply (drule spec[where x=co_ctx])
-  apply clarsimp
   apply (drule spec2[where x=presult and y="R ** rest"])
   apply (simp add:sep_conj_ac )
   done
@@ -846,7 +886,6 @@ lemma weaken_post:
   apply clarsimp
   subgoal for co_ctx presult rest stopper
   apply (drule spec[where x=co_ctx])
-  apply clarsimp
   apply (drule spec2[where x=presult and y=rest])
   apply clarsimp
   apply (drule spec[where x=stopper])
@@ -865,7 +904,6 @@ lemma strengthen_pre:
   apply (simp add: triple_def)
   apply(clarify)
   apply(drule_tac x = co_ctx in spec)
-  apply(simp)
   apply(drule_tac x = presult in spec)
   apply(drule_tac x = rest in spec)
   apply simp
@@ -965,7 +1003,6 @@ shows" triple net reasons b c q"
 using assms(2)
   apply(auto simp add: triple_def)
   apply(drule_tac x = co_ctx in spec)
-  apply(auto)
   apply(drule_tac x = presult in spec)
   apply(drule_tac x = rest in spec)
   apply (erule impE)
@@ -997,7 +1034,6 @@ declare sep_code_sep [simp del]
 lemma preE : "triple net reasons (\<lambda> s. \<exists> x. p x s) c q = (\<forall> x. triple net reasons (p x) c q)"
 apply(auto simp add: triple_def)
  apply(erule_tac x = co_ctx in allE)
- apply simp
  apply(drule_tac x = presult in spec)
   apply(drule_tac x = rest in spec)
   apply (erule impE)
